fairneris/aneris_lang/state_interp/state_interp_config_wp.v
@@ -1,6 +1,6 @@
 From iris.proofmode Require Import tactics.
 From trillium.program_logic Require Export adequacy.
-From fairneris Require Import fuel.
+From fairneris Require Import fuel env_model.
 From fairneris.aneris_lang Require Import
      aneris_lang network resources.
 From fairneris.prelude Require Import gmultiset.
@@ -24,7 +24,7 @@ Import uPred.
 Import RecordSetNotations.
 
 Section state_interpretation.
-  Context `{LM: LiveModel aneris_lang Mod}.
+  Context `{LM: LiveModel aneris_lang (joint_model Mod Net)}.
   Context `{aG : !anerisG LM Σ}.
 
   (* TODO: Move this elsehwere and use it where we now use ad hoc induction *)
@@ -128,117 +128,117 @@ Section state_interpretation.
   (*TODO: lots of copy pasta! *)
   Lemma config_wp_correct : ⊢ config_wp.
   Proof.
-    rewrite /config_wp. iModIntro.
-    iIntros (ex atr c lbl σ2 Hexvalid Hex Hstep) "(% & Hsi & Hlive & Hauth)".
-    rewrite (last_eq_trace_ends_in ex c); [|done].
-    rewrite /aneris_state_interp.
-    iDestruct "Hsi" as (γm mh)
-                         "(%Hhist & %Hgcoh & %Hnscoh & %Hmhcoh &
-                           Hnauth & Hsi & Hlcoh & Hfreeips & Hmctx & Hmres)".
-    iMod (steps_auth_update_S with "Hauth") as "Hauth".
-    iApply fupd_elim_laterN; [solve_ndisj|].
-    destruct c as [tp1 σ1]=> /=.
-    rewrite /valid_state_evolution_fairness in H.
-    rewrite /trace_ends_in in Hex.
-    have Hlstep: locale_step (tp1, σ1) (inr lbl) (tp1, σ2) by econstructor.
-    destruct σ1; simpl in *; simplify_eq.
-    pose (trace_last atr) as δ.
-    inversion Hstep as
-      [ip σ Sn Sn' sh a skt R m Hm HSn Hsh HSn' Hsaddr|
-        σ|
-        σ];
-      simplify_eq/=.
-    (* Deliver *)
-    - destruct H as (Hsteps & Hmatch & Htids).
-      destruct (LM.(lm_cfg_action) (trace_last atr) (Some m)) as [ℓ δ'] eqn:Heq.
-      unshelve iExists ({| ls_data := {| ls_under := δ'; ls_map := δ.(ls_data).(ls_map) |} |}).
-      { admit. }
-      { admit. }
-      iExists (Config_step ℓ (Some m : config_label aneris_lang)).
-      iSplitR.
-      { iPureIntro.
-        rewrite /valid_state_evolution_fairness.
-        rewrite /messages_to_receive_at_multi_soup in Hm.
-        split.
-        { econstructor; [done|econstructor|done]; simpl.
-          - by eapply lm_cfg_spec_trans.
-          - split=>//. by eapply lm_cfg_spec_live_roles. }
-        split; first (split; [done|by eapply lm_cfg_spec_labels_match]).
-        by rewrite /tids_smaller ?Hex //= in Htids *. }
-      iFrame "Hauth". simpl.
-      iDestruct "Hlive" as "(#Hupd&%fm&?&?&?&Hst&?)".
-      iMod ("Hupd" $! _ _ _ _ Heq with "Hst").
-      iModIntro. iSplitL "Hnauth Hsi Hlcoh Hfreeips Hmctx Hmres"; last first.
-      { iSplit; iFrame "#". iExists fm. erewrite lm_cfg_spec_live_roles=>//. iFrame. }
-      iExists γm, mh. iFrame.
-      iSplit.
-      { apply (last_eq_trace_ends_in) in Hex as ->.
-        erewrite <- message_history_evolution_deliver_message;
-          eauto with set_solver. }
-      iSplitR; [eauto using gnames_coh_update_sockets|].
-      assert (m_destination m = a) by set_solver. (* TODO: Remove filter thing *)
-      iSplitR; [eauto using network_sockets_coh_deliver_message|].
-      iSplitR; [iPureIntro; apply messages_history_coh_drop_message;
-                eauto using messages_history_coh_deliver_message|].
-      iSplitL "Hlcoh";
-        [by iApply (local_state_coh_deliver_message with "Hlcoh")|].
-      by iApply (free_ips_coh_deliver_message with "Hfreeips").
-    - destruct H as (Hsteps & Hmatch & Htids).
-      destruct (LM.(lm_cfg_action) (trace_last atr) None) as [ℓ δ'] eqn:Heq.
-      unshelve iExists ({| ls_data := {| ls_under := δ'; ls_map := δ.(ls_data).(ls_map) |} |}).
-      { admit. }
-      { admit. }
-      iExists (Config_step ℓ (None : config_label aneris_lang)).
-      iSplitR.
-      { iPureIntro.
-        rewrite /valid_state_evolution_fairness.
-        split.
-        { econstructor; [done|econstructor|done]; simpl.
-          - by eapply lm_cfg_spec_trans.
-          - split=>//. by eapply lm_cfg_spec_live_roles. }
-        split; first (split; [done|by eapply lm_cfg_spec_labels_match]).
-        by rewrite /tids_smaller ?Hex //= in Htids *. }
-      iFrame "Hauth". simpl.
-      iDestruct "Hlive" as "(#Hupd&%fm&?&?&?&Hst&?)".
-      iMod ("Hupd" $! _ _ _ _ Heq with "Hst").
-      iModIntro. iSplitL "Hnauth Hsi Hlcoh Hfreeips Hmctx Hmres"; last first.
-      { iSplit; iFrame "#". iExists fm. erewrite lm_cfg_spec_live_roles=>//. iFrame. }
-      iExists γm, mh. iFrame.
-      iSplit.
-      { apply (last_eq_trace_ends_in) in Hex as ->.
-        erewrite <- message_history_evolution_duplicate_message;
-          eauto with set_solver. multiset_solver. }
-      iSplitR; [eauto using gnames_coh_update_sockets|].
-      iSplitR; [eauto using network_sockets_coh_deliver_message|].
-      eauto using messages_history_coh_duplicate_message.
-    - destruct H as (Hsteps & Hmatch & Htids).
-      destruct (LM.(lm_cfg_action) (trace_last atr) None) as [ℓ δ'] eqn:Heq.
-      unshelve iExists ({| ls_data := {| ls_under := δ'; ls_map := δ.(ls_data).(ls_map) |} |}).
-      { admit. }
-      { admit. }
-      iExists (Config_step ℓ (None : config_label aneris_lang)).
-      iSplitR.
-      { iPureIntro.
-        rewrite /valid_state_evolution_fairness.
-        split.
-        { econstructor; [done|econstructor|done]; simpl.
-          - by eapply lm_cfg_spec_trans.
-          - split=>//. by eapply lm_cfg_spec_live_roles. }
-        split; first (split; [done|by eapply lm_cfg_spec_labels_match]).
-        by rewrite /tids_smaller ?Hex //= in Htids *. }
-      iFrame "Hauth". simpl.
-      iDestruct "Hlive" as "(#Hupd&%fm&?&?&?&Hst&?)".
-      iMod ("Hupd" $! _ _ _ _ Heq with "Hst").
-      iModIntro. iSplitL "Hnauth Hsi Hlcoh Hfreeips Hmctx Hmres"; last first.
-      { iSplit; iFrame "#". iExists fm. erewrite lm_cfg_spec_live_roles=>//. iFrame. }
-      iExists γm, mh. iFrame.
-      iSplit.
-      { apply (last_eq_trace_ends_in) in Hex as ->.
-        erewrite <- message_history_evolution_drop_message;
-          eauto with set_solver. multiset_solver. }
-      iSplitR; [eauto using gnames_coh_update_sockets|].
-      iSplitR; [eauto using network_sockets_coh_deliver_message|].
-      eauto using messages_history_coh_drop_message.
+    (* rewrite /config_wp. iModIntro. *)
+    (* iIntros (ex atr c lbl σ2 Hexvalid Hex Hstep) "(% & Hsi & Hlive & Hauth)". *)
+    (* rewrite (last_eq_trace_ends_in ex c); [|done]. *)
+    (* rewrite /aneris_state_interp. *)
+    (* iDestruct "Hsi" as (γm mh) *)
+    (*                      "(%Hhist & %Hgcoh & %Hnscoh & %Hmhcoh & *)
+    (*                        Hnauth & Hsi & Hlcoh & Hfreeips & Hmctx & Hmres)". *)
+    (* iMod (steps_auth_update_S with "Hauth") as "Hauth". *)
+    (* iApply fupd_elim_laterN; [solve_ndisj|]. *)
+    (* destruct c as [tp1 σ1]=> /=. *)
+    (* rewrite /valid_state_evolution_fairness in H. *)
+    (* rewrite /trace_ends_in in Hex. *)
+    (* have Hlstep: locale_step (tp1, σ1) (inr lbl) (tp1, σ2) by econstructor. *)
+    (* destruct σ1; simpl in *; simplify_eq. *)
+    (* pose (trace_last atr) as δ. *)
+    (* inversion Hstep as *)
+    (*   [ip σ Sn Sn' sh a skt R m Hm HSn Hsh HSn' Hsaddr| *)
+    (*     σ| *)
+    (*     σ]; *)
+    (*   simplify_eq/=. *)
+    (* (* Deliver *) *)
+    (* - destruct H as (Hsteps & Hmatch & Htids). *)
+    (*   destruct (LM.(lm_cfg_action) (trace_last atr) (Some m)) as [ℓ δ'] eqn:Heq. *)
+    (*   unshelve iExists ({| ls_data := {| ls_under := δ'; ls_map := δ.(ls_data).(ls_map) |} |}). *)
+    (*   { admit. } *)
+    (*   { admit. } *)
+    (*   iExists (Config_step ℓ (Some m : config_label aneris_lang)). *)
+    (*   iSplitR. *)
+    (*   { iPureIntro. *)
+    (*     rewrite /valid_state_evolution_fairness. *)
+    (*     rewrite /messages_to_receive_at_multi_soup in Hm. *)
+    (*     split. *)
+    (*     { econstructor; [done|econstructor|done]; simpl. *)
+    (*       - by eapply lm_cfg_spec_trans. *)
+    (*       - split=>//. by eapply lm_cfg_spec_live_roles. } *)
+    (*     split; first (split; [done|by eapply lm_cfg_spec_labels_match]). *)
+    (*     by rewrite /tids_smaller ?Hex //= in Htids *. } *)
+    (*   iFrame "Hauth". simpl. *)
+    (*   iDestruct "Hlive" as "(#Hupd&%fm&?&?&?&Hst&?)". *)
+    (*   iMod ("Hupd" $! _ _ _ _ Heq with "Hst"). *)
+    (*   iModIntro. iSplitL "Hnauth Hsi Hlcoh Hfreeips Hmctx Hmres"; last first. *)
+    (*   { iSplit; iFrame "#". iExists fm. erewrite lm_cfg_spec_live_roles=>//. iFrame. } *)
+    (*   iExists γm, mh. iFrame. *)
+    (*   iSplit. *)
+    (*   { apply (last_eq_trace_ends_in) in Hex as ->. *)
+    (*     erewrite <- message_history_evolution_deliver_message; *)
+    (*       eauto with set_solver. } *)
+    (*   iSplitR; [eauto using gnames_coh_update_sockets|]. *)
+    (*   assert (m_destination m = a) by set_solver. (* TODO: Remove filter thing *) *)
+    (*   iSplitR; [eauto using network_sockets_coh_deliver_message|]. *)
+    (*   iSplitR; [iPureIntro; apply messages_history_coh_drop_message; *)
+    (*             eauto using messages_history_coh_deliver_message|]. *)
+    (*   iSplitL "Hlcoh"; *)
+    (*     [by iApply (local_state_coh_deliver_message with "Hlcoh")|]. *)
+    (*   by iApply (free_ips_coh_deliver_message with "Hfreeips"). *)
+    (* - destruct H as (Hsteps & Hmatch & Htids). *)
+    (*   destruct (LM.(lm_cfg_action) (trace_last atr) None) as [ℓ δ'] eqn:Heq. *)
+    (*   unshelve iExists ({| ls_data := {| ls_under := δ'; ls_map := δ.(ls_data).(ls_map) |} |}). *)
+    (*   { admit. } *)
+    (*   { admit. } *)
+    (*   iExists (Config_step ℓ (None : config_label aneris_lang)). *)
+    (*   iSplitR. *)
+    (*   { iPureIntro. *)
+    (*     rewrite /valid_state_evolution_fairness. *)
+    (*     split. *)
+    (*     { econstructor; [done|econstructor|done]; simpl. *)
+    (*       - by eapply lm_cfg_spec_trans. *)
+    (*       - split=>//. by eapply lm_cfg_spec_live_roles. } *)
+    (*     split; first (split; [done|by eapply lm_cfg_spec_labels_match]). *)
+    (*     by rewrite /tids_smaller ?Hex //= in Htids *. } *)
+    (*   iFrame "Hauth". simpl. *)
+    (*   iDestruct "Hlive" as "(#Hupd&%fm&?&?&?&Hst&?)". *)
+    (*   iMod ("Hupd" $! _ _ _ _ Heq with "Hst"). *)
+    (*   iModIntro. iSplitL "Hnauth Hsi Hlcoh Hfreeips Hmctx Hmres"; last first. *)
+    (*   { iSplit; iFrame "#". iExists fm. erewrite lm_cfg_spec_live_roles=>//. iFrame. } *)
+    (*   iExists γm, mh. iFrame. *)
+    (*   iSplit. *)
+    (*   { apply (last_eq_trace_ends_in) in Hex as ->. *)
+    (*     erewrite <- message_history_evolution_duplicate_message; *)
+    (*       eauto with set_solver. multiset_solver. } *)
+    (*   iSplitR; [eauto using gnames_coh_update_sockets|]. *)
+    (*   iSplitR; [eauto using network_sockets_coh_deliver_message|]. *)
+    (*   eauto using messages_history_coh_duplicate_message. *)
+    (* - destruct H as (Hsteps & Hmatch & Htids). *)
+    (*   destruct (LM.(lm_cfg_action) (trace_last atr) None) as [ℓ δ'] eqn:Heq. *)
+    (*   unshelve iExists ({| ls_data := {| ls_under := δ'; ls_map := δ.(ls_data).(ls_map) |} |}). *)
+    (*   { admit. } *)
+    (*   { admit. } *)
+    (*   iExists (Config_step ℓ (None : config_label aneris_lang)). *)
+    (*   iSplitR. *)
+    (*   { iPureIntro. *)
+    (*     rewrite /valid_state_evolution_fairness. *)
+    (*     split. *)
+    (*     { econstructor; [done|econstructor|done]; simpl. *)
+    (*       - by eapply lm_cfg_spec_trans. *)
+    (*       - split=>//. by eapply lm_cfg_spec_live_roles. } *)
+    (*     split; first (split; [done|by eapply lm_cfg_spec_labels_match]). *)
+    (*     by rewrite /tids_smaller ?Hex //= in Htids *. } *)
+    (*   iFrame "Hauth". simpl. *)
+    (*   iDestruct "Hlive" as "(#Hupd&%fm&?&?&?&Hst&?)". *)
+    (*   iMod ("Hupd" $! _ _ _ _ Heq with "Hst"). *)
+    (*   iModIntro. iSplitL "Hnauth Hsi Hlcoh Hfreeips Hmctx Hmres"; last first. *)
+    (*   { iSplit; iFrame "#". iExists fm. erewrite lm_cfg_spec_live_roles=>//. iFrame. } *)
+    (*   iExists γm, mh. iFrame. *)
+    (*   iSplit. *)
+    (*   { apply (last_eq_trace_ends_in) in Hex as ->. *)
+    (*     erewrite <- message_history_evolution_drop_message; *)
+    (*       eauto with set_solver. multiset_solver. } *)
+    (*   iSplitR; [eauto using gnames_coh_update_sockets|]. *)
+    (*   iSplitR; [eauto using network_sockets_coh_deliver_message|]. *)
+    (*   eauto using messages_history_coh_drop_message. *)
   Admitted.
 
 End state_interpretation.
